defining top level compiler lemmas

compiler.v
@@ -1,16 +1,16 @@
 Require expr cbn cem cesm im db assembly.
-Require cbn_cem cem_cesm.
+Require cem_cesm cesm_im.
 Require Import Unicode.Utf8.
-Require Import util expr_db db_assembly.
+Require Import util expr_db db_assembly relations.
 
 (* This file has the high level structure of the compiler and the corresponding
 main theorems of correctness *)
 
-Definition compile (t : expr.tm) : option assembly.Program := match db t nil with
-  | Some a => Some (assemble a 0)
-  | None => None 
-  end.
+Definition compile t := assemble t 0.
 
+Theorem compile_correct (t : db.tm) : db.closed t → cem.step (cem.I t) v → 
+  { mv : im.State | refl_trans_clos im.step (im.I (compile t)) mv *
+                    state_rel (cesm.st mv cem.st_h } 
 (*Theorem compile_correct : Type := bool.
  Definition compile (t: expr.tm) : expr.closed t → { mc | trans_clos prog p }.
 *)
